\documentclass[a4paper,11pt]{article}
\usepackage{amsmath}
% define the title
\author{John Hancock}
\title{Udacity Intro To Statistics Problem Set 6}
\begin{document}
% generates the title
\maketitle
% insert the table of contents
\tableofcontents
\section{Ratio of Correlation to Regression}
Given:

\begin{equation}
b = 
  \frac{ \sum_{i=1}^n \left(x_i - \bar{x}\right)\left(y_i - \bar{y}\right) } 
    { \sum_{i=1}^n \left(x_i - \bar{x} \right)^2 }
\end{equation}

and:

\begin{equation}
r = 
  \frac{ \sum_{i=1}^n \left(x_i - \bar{x}\right)\left(y_i - \bar{y}\right) }
   { \sqrt{\sum_{i=1}^n \left(x_i - \bar{x} \right)^2 
      \sum_{i=1}^n \left(y_i - \bar{y} \right)^2 } }
\end{equation}

find a simplified form for $\frac{b}{r}$

let $f\left( x \right ) = $

\begin{equation}
  \sum_{i=1}^n \left(x_i - \bar{x}\right)\left(y_i - \bar{y}\right) 
\end{equation}

then $\frac{b}{r} = $

\begin{equation}
  \frac{ 
    \frac { f \left(x\right) } { \sum_{i=1}^n \left(x_i - \bar{x} \right)^2 }
    }
    {\frac 
      { f \left(x\right) }
      {
        \sqrt{\sum_{i=1}^n \left(x_i - \bar{x} \right)^2 
        \sum_{i=1}^n \left(y_i - \bar{y} \right)^2 } 
      }
    }
\end{equation}


\begin{equation}
\implies
\frac{b}{r} = 
  \frac { f \left(x\right) } { \sum_{i=1}^n \left(x_i - \bar{x} \right)^2 }
  \frac  {
        \sqrt{\sum_{i=1}^n \left(x_i - \bar{x} \right)^2 
        \sum_{i=1}^n \left(y_i - \bar{y} \right)^2 } 
      }
      { f \left(x\right) }
\end{equation}

\begin{equation}
\implies
\frac{b}{r} = 
  \frac
    {
      \sqrt{\sum_{i=1}^n \left(x_i - \bar{x} \right)^2 
      \sum_{i=1}^n \left(y_i - \bar{y} \right)^2 } 
    }
    {
      \sum_{i=1}^n \left(x_i - \bar{x} \right)^2 
    }
\end{equation}


\begin{equation}
\implies
\frac{b}{r} = 
  \frac
    {
      \sqrt{\sum_{i=1}^n \left(x_i - \bar{x} \right)^2}
      \sqrt{\sum_{i=1}^n \left(y_i - \bar{y} \right)^2 } 
    }
    {
      \sum_{i=1}^n \left(x_i - \bar{x} \right)^2 
    }
\end{equation}

\begin{equation}
\implies
\frac{b}{r} = 
  \frac
    {
      (\sum_{i=1}^n \left(x_i - \bar{x} \right)^2)^\frac{1}{2}
      \sqrt{\sum_{i=1}^n \left(y_i - \bar{y} \right)^2 } 
    }
    {
      \sum_{i=1}^n \left(x_i - \bar{x} \right)^2 
    }
\end{equation}

\begin{equation}
\implies
\frac{b}{r} = 
\left( \sum_{i=1}^n \left(x_i - \bar{x} \right)^2 \right) ^ \frac{1}{2}
\left( \sum_{i=1}^n \left(x_i - \bar{x} \right)^2 \right) ^ {-1}
\sqrt{\sum_{i=1}^n \left(y_i - \bar{y} \right)^2 }
\end{equation}

\begin{equation}
\implies
\frac{b}{r} = 
\left( \sum_{i=1}^n \left(x_i - \bar{x} \right)^2 \right) ^ {-\frac{1}{2}}
\sqrt{\sum_{i=1}^n \left(y_i - \bar{y} \right)^2 }
\end{equation}


\begin{equation}
\implies
\frac{b}{r} = 
\frac
{\sqrt{\sum_{i=1}^n \left(y_i - \bar{y} \right)^2 }}
{\sqrt{\left( \sum_{i=1}^n \left(x_i - \bar{x} \right)^2 \right)} }
\end{equation}


\begin{equation}
\implies
\frac{b}{r} = 
\sqrt{
  \frac
    {\sum_{i=1}^n \left(y_i - \bar{y} \right)^2}
    {\sum_{i=1}^n \left(x_i - \bar{x} \right)^2}
  }
\end{equation}

\end{document}
